

# Correction: Proof of the Microstructure/Gluing Estimate (prop:glue-gap)

This note provides a self-contained corrected proof of the “Microstructure/gluing estimate” as it appears in `Hodge-v6-w-Jon-Update-MERGED.tex` (Proposition `\ref{prop:glue-gap}`). The issue in the manuscript version is purely in the *written proof* of the proposition: the statement already contains the correct bound (displacement  $\times$  slice mass), but the short proof sketch incorrectly drops the slice-mass factor and references boundary faces rather than interior interfaces.

## Minimal background

We use only the standard “flat norm” inequality: if  $T$  is a current and  $Q$  is any current with  $\partial Q = T$ , then

$$\mathcal{F}(T) \leq \text{Mass}(Q),$$

since one may take  $R = 0$  in the definition  $\mathcal{F}(T) = \inf\{\text{Mass}(R) + \text{Mass}(Q) : T = R + \partial Q\}$ .

## Translation filling lemma

**Lemma 1** (Flat-norm stability under translation). *Let  $S$  be an integral  $\ell$ -cycle in  $\mathbb{R}^d$  (so  $\partial S = 0$ ) with finite mass. For any translation vector  $v \in \mathbb{R}^d$ , let  $\tau_v(x) = x + v$  and  $(\tau_v)_\# S$  be the pushforward. Then there exists an integral  $(\ell + 1)$ -current  $Q$  such that*

$$\partial Q = (\tau_v)_\# S - S, \quad \text{Mass}(Q) \leq \|v\| \text{Mass}(S).$$

*Proof.* Let  $H : [0, 1] \times \mathbb{R}^d \rightarrow \mathbb{R}^d$  be the straight-line homotopy  $H(t, x) = x + tv$ . Define  $Q := H_\#([0, 1] \times S)$ . Since  $\partial([0, 1] \times S) = \{1\} \times S - \{0\} \times S - [0, 1] \times \partial S$  and  $\partial S = 0$ , we have  $\partial Q = (\tau_v)_\# S - S$ . The map  $H$  has Jacobian bounded by  $\|v\|$  in the  $t$ -direction, hence  $\text{Mass}(Q) \leq \|v\| \text{Mass}(S)$ .  $\square$

## Corrected gluing estimate

**Proposition 1** (Microstructure/gluing estimate (corrected proof)). *Let  $k \geq 1$  and let*

$$T^{\text{raw}} = \sum_Q S_Q$$

*be an integral  $k$ -current obtained by summing integral  $k$ -currents  $S_Q$  supported on cells  $Q$  of a cubulation. Assume the boundary admits an oriented face decomposition*

$$\partial T^{\text{raw}} = \sum_F B_F$$

as a sum over interior interfaces  $F = Q \cap Q'$  where each face mismatch is

$$B_F = (\partial S_Q)_\perp F - (\partial S_{Q'})_\perp F.$$

Assume moreover that for each interface  $F$  there exist cycle slices  $\Sigma_F(u)$  on  $F$  depending on  $u \in \Omega_F \subset \mathbb{R}^{2p}$  such that:

- for some multisets  $\{u_{F,a}\}_{a=1}^{N_F}$  and  $\{u'_{F,a}\}_{a=1}^{N_F}$ ,

$$B_F = \sum_{a=1}^{N_F} \Sigma_F(u_{F,a}) - \sum_{a=1}^{N_F} \Sigma_F(u'_{F,a});$$

- in face coordinates, each  $\Sigma_F(u)$  is obtained from  $\Sigma_F(0)$  by translation by  $u$ ;
- there exists a matching  $\sigma_F \in S_{N_F}$  with a uniform displacement bound

$$\|u_{F,a} - u'_{F,\sigma_F(a)}\| \leq \Delta_F \quad \text{for all } a.$$

Define, for each  $F$  and  $a$ , the translation vector  $v_{F,a} := u'_{F,\sigma_F(a)} - u_{F,a}$  and let  $Q_{F,a}$  be the integral  $k$ -current provided by Lemma 1 applied (in the face chart) to the  $(k-1)$ -cycle  $\Sigma_F(u_{F,a})$ , so that

$$\partial Q_{F,a} = \Sigma_F(u_{F,a}) - \Sigma_F(u'_{F,\sigma_F(a)}), \quad \text{Mass}(Q_{F,a}) \leq \|v_{F,a}\| \text{Mass}(\Sigma_F(u_{F,a})).$$

Set

$$Q_F := \sum_{a=1}^{N_F} Q_{F,a}, \quad U := \sum_F Q_F, \quad T := T^{\text{raw}} - U.$$

Then:

- $U$  is an integral  $k$ -current and  $\partial U = \partial T^{\text{raw}}$ , hence  $T$  is an integral  $k$ -cycle.
- The mass of  $U$  satisfies

$$\text{Mass}(U) \leq \sum_F \text{Mass}(Q_F) \leq \sum_F \Delta_F \sum_{a=1}^{N_F} \text{Mass}(\Sigma_F(u_{F,a})).$$

- In particular,

$$\mathcal{F}(\partial T^{\text{raw}}) \leq \text{Mass}(U).$$

*Proof.* Fix an interface  $F$  and its matching  $\sigma_F$ . Summing the boundary identities for  $Q_{F,a}$  gives

$$\partial Q_F = \sum_{a=1}^{N_F} (\Sigma_F(u_{F,a}) - \Sigma_F(u'_{F,\sigma_F(a)})) = B_F.$$

Summing over all interfaces yields

$$\partial U = \sum_F \partial Q_F = \sum_F B_F = \partial T^{\text{raw}},$$

so  $T = T^{\text{raw}} - U$  is a cycle.

For the mass bound, by the triangle inequality and the estimate from Lemma 1,

$$\text{Mass}(Q_F) \leq \sum_{a=1}^{N_F} \text{Mass}(Q_{F,a}) \leq \sum_{a=1}^{N_F} \|u_{F,a} - u'_{F,\sigma_F(a)}\| \text{Mass}(\Sigma_F(u_{F,a})) \leq \Delta_F \sum_{a=1}^{N_F} \text{Mass}(\Sigma_F(u_{F,a})).$$

Summing over  $F$  gives (ii). Finally, since  $\partial U = \partial T^{\text{raw}}$ , taking  $Q := U$  and  $R := 0$  in the flat norm definition yields  $\mathcal{F}(\partial T^{\text{raw}}) \leq \text{Mass}(U)$ , proving (iii).  $\square$